Algdata/Data/Array/Basic.lean
@@ -1,0 +1,350 @@
+/-
+Copyright (c) 2022 Jun Yoshida. All rights reserved.
+Released under Apache 2.0 license as described in the file LICENSE.
+-/
+
+import Std.Data.Array.Lemmas
+
+/-!
+# Auxiliary functions not in the core and `Std`
+
+More auxiliary lemmas are found in `Algdata.Data.Array.Lemmas`.
+
+## TODO
+
+* Give the specification theorem to `Array.anyIdxM` and `Array.anyIdx`.
+
+-/
+
+-- Disable auto-binding of unbounded variables
+set_option autoImplicit false
+
+universe u v
+
+
+namespace Array
+
+variable {α : Type u} {β : Type v}
+
+/-!
+### Declaration about `Array.cons`
+-/
+
+section Cons
+
+/--
+An `Array` counterpart of `List.cons`.
+
+:::note warning
+In view of performance, construction based on `Array.push` is preferred.
+:::
+-/
+def cons (a : α) (as : Array α) : Array α :=
+  ⟨a :: as.data⟩
+
+@[simp]
+theorem data_cons (a : α) (as : Array α) : Array.data (cons a as) = a :: as.data :=
+  rfl
+
+@[simp]
+theorem size_cons (a : α) (as : Array α) : Array.size (cons a as) = as.size.succ :=
+  rfl
+
+theorem push_empty_eq_cons (a : α) : push #[] a = cons a #[] :=
+  rfl
+
+theorem push_cons_eq_cons_push (a b : α) (as : Array α) : push (cons a as) b = cons a (push as b) := by
+  dsimp [push, cons, List.concat]
+
+@[simp]
+theorem getElem_cons_zero {a : α} {x : Array α} : (cons a x)[0]'(x.size.zero_lt_succ) = a :=
+  rfl
+
+@[simp]
+theorem getElem_cons_succ {a : α} {x : Array α} (i : Nat) (hi : i+1 < x.size+1) : (cons a x)[i+1]'hi = x[i]'(Nat.lt_of_succ_lt_succ hi) :=
+  rfl
+
+/-- Induction step for `Array` based on `Array.empty` (aka `#[]`) and `Array.cons`. -/
+@[elab_as_elim]
+theorem cons_induction
+    {motive : Array α → Prop}
+    (empty : motive #[])
+    (cons : ∀ (a : α) (x : Array α), motive x → motive (cons a x))
+    (x : Array α)
+  : motive x :=
+  x.rec $ List.rec empty λ a as IH => cons a ⟨as⟩ IH
+
+/-- Induction step for `Array` based on `Array.empty` (aka `#[]`) and `Array.cons`. The version takes the major premise as the first argument. -/
+@[elab_as_elim]
+theorem cons_induction_on
+    {motive : Array α → Prop}
+    (x : Array α)
+    (empty : motive #[])
+    (cons : ∀ (a : α) (x : Array α), motive x → motive (cons a x))
+  : motive x :=
+  x.cons_induction empty cons
+
+/-- Case-splitting for `Array` into `Array.empty` (aka `#[]`) and `Array.cons`. -/
+@[elab_as_elim]
+theorem cons_cases_on
+    {motive : Array α → Prop}
+    (x : Array α)
+    (empty : motive #[])
+    (cons : ∀ (a : α) (x : Array α), motive (cons a x))
+  : motive x :=
+  x.cons_induction empty fun a x _ => cons a x
+
+end Cons
+
+
+/-! ### Declarations about `Array.back'` -/
+
+section Back
+
+/-- `back' as h` is the last entry of `as : Array α` with `h : as.size > 0`. In contrast to `Array.back`, this function does not require `Inhabited α` since it doesn't fail thanks to `h`. -/
+def back' (as : Array α) (h : as.size > 0) : α :=
+  have : as.size - 1 < as.size := Nat.pred_lt' h
+  as[as.size - 1]' this
+
+/-- `Array.back'` is a counterpart of `List.getLast`. -/
+theorem back'_eq_data_getLast (as : Array α) (h : as.size > 0) : as.back' h = as.data.getLast (h |> as.casesOn λ l (h : l.length > 0) (hc : l = []) => by cases hc; cases h) := by
+  rw [List.getLast_eq_get]; rfl
+
+end Back
+
+
+/-! ### Variants of `Array.any` -/
+
+section Any
+
+variable {m : Type → Type v} [Monad m]
+
+/--
+`Array.anyIdxM x p start stop` checks if there is an element in `x : Array α` with indices `start ≤ i < stop` satisfying an index-dependent `Bool`-valued predicate `p : Fin x.size → α → m Bool`.
+The last two arguments are optional; the default values are `start := 0` and `stop := x.size`.
+This is an index-dependent analogue of `Array.anyM` and a bit less efficient in runtime.
+-/
+@[inline]
+def anyIdxM (x : Array α) (p : Fin x.size → α → m Bool) (start := 0) (stop := x.size) : m Bool :=
+  let any (stop : Nat) (h : stop ≤ x.size) :=
+    let rec @[specialize] loop (i : Nat) : m Bool := do
+      if hlt : i < stop then
+        have : i < x.size := trans hlt h
+        if (← p ⟨i,this⟩ x[i]) then
+          return true
+        else
+          loop (i+1)
+      else
+        return false
+    loop start
+  if h : stop ≤ x.size then
+    any stop h
+  else
+    any x.size .refl
+termination_by loop i => stop - i
+
+/--
+`Array.anyIdx x p start stop` checks if there is an element in `x : Array α` with indices `start ≤ i < stop` satisfying an index-dependent `Bool`-valued predicate `p : Fin x.size → α → Bool`.
+The last two arguments are optional; the default values are `start := 0` and `stop := x.size`.
+This is an index-dependent analogue of `Array.any` and a bit less effieicnet in runtime.
+If `p` has values in a monad context, use `Array.anyIdxM` instead.
+-/
+@[inline]
+def anyIdx (x : Array α) (p : Fin x.size → α → Bool) (start := 0) (stop := x.size) : Bool :=
+  Id.run <| x.anyIdxM p start stop
+
+/-- The runtime implementation of `Array.anyPairM`. -/
+@[inline]
+unsafe def anyPairMUnsafe (x : Array α) (p : α → α → m Bool) (start := 0) (stop := x.size) : m Bool := do
+  let rec @[specialize] any (i j : USize) (stop : USize) : m Bool := do
+    if j == stop then
+      let i := i + 1
+      if i == stop then
+        return false
+      else
+        any i (i+1) stop
+    else
+      if (← p (x.uget i lcProof) (x.uget j lcProof)) then
+        return true
+      else
+        any i (j+1) stop
+  let start := USize.ofNat start
+  let stop := USize.ofNat <| min stop x.size
+  if start < stop then
+    any start (start+1) stop
+  else
+    return false
+
+/--
+`Array.anyPairM x p start stop` check is there is an ordered pair of elements `(x[i],x[j])` in `x : Array α` with indices `start ≤ i < j < stop` satisfying a given `Bool`-valued binary predicate `p : α → α → m Bool` in a monad context.
+The last two arguments are optional; the default values are `start := 0` and `stop := x.size`.
+-/
+@[implemented_by anyPairMUnsafe]
+def anyPairM (x : Array α) (p : α → α → m Bool) (start : Nat := 0) (stop : Nat := x.size) : m Bool := do
+  let any (stop : Nat) (h : stop ≤ x.size) :=
+    let rec loop (i j : Nat) (hij : i < j) : m Bool := do
+      if hj : j < stop then
+        have : i < x.size := trans (trans hij hj) h
+        have : j < x.size := trans hj h
+        if (← p x[i] x[j]) then
+          return true
+        else
+          loop i (j+1) (.step hij)
+      else
+        if i < stop then
+          loop (i+1) (i+2) (i+1).lt_succ_self
+        else
+          return false
+    loop start (start+1) start.lt_succ_self
+  if h : stop ≤ x.size then
+    any stop h
+  else
+    any x.size .refl
+termination_by loop i j _ => (stop - i, stop - j)
+
+/--
+`Array.anyPair x p start stop` check is there is an ordered pair of elements `(x[i],x[j])` in `x : Array α` with indices `start ≤ i < j < stop` satisfying a given `Bool`-valued binary predicate `p : α → α → Bool`.
+The last two arguments are optional; the default values are `start := 0` and `stop := x.size`.
+This function is thought of as the `Bool`-valued `Array`-analogue of `List.Pairwise`.
+See also `Array.anyPairM`.
+-/
+@[inline]
+def anyPair (x : Array α) (p : α → α → Bool) (start : Nat := 0) (stop : Nat := x.size) : Bool :=
+  Id.run <| x.anyPairM p start stop
+
+theorem anyPairM_loop_empty (p : α → α → m Bool) {stop : Nat} (h : stop ≤ 0) {i j : Nat} (hij : i < j) : anyPairM.loop #[] p stop h i j hij = pure false := by
+  cases Nat.eq_zero_of_le_zero h
+  unfold anyPairM.loop
+  rw [dif_neg j.not_lt_zero, if_neg i.not_lt_zero]
+
+theorem anyPairM_loop_cons_succ (a : α) (x : Array α) (p : α → α → m Bool) {stop : Nat} (h : stop ≤ x.size) {i j : Nat} (hij : i < j)
+  : anyPairM.loop (cons a x) p (stop + 1) (Nat.succ_le_succ h) (i+1) (j+1) (Nat.succ_lt_succ hij) = anyPairM.loop x p stop h i j hij := by
+  unfold anyPairM.loop
+  if hj : j < stop then
+    rewrite [dif_pos (Nat.succ_lt_succ hj), dif_pos hj]
+    apply bind_congr; intro b
+    match b with
+    | true => rfl
+    | false =>
+      simp only [ite_false]
+      exact anyPairM_loop_cons_succ a x p h (.step hij)
+  else
+    rewrite [dif_neg (fun h' => hj (Nat.lt_of_succ_lt_succ h')), dif_neg hj]
+    if hi : i < stop then
+      rewrite [if_pos (Nat.succ_lt_succ hi), if_pos hi]
+      exact anyPairM_loop_cons_succ a x p h (i+1).lt_succ_self
+    else
+      rw [if_neg (fun h' => hi (Nat.lt_of_succ_lt_succ h')), if_neg hi]
+termination_by _ => (stop - i, stop - j)
+
+theorem anyPairM_loop_cons_zero [LawfulMonad m] (a : α) (x : Array α) (p : α → α → m Bool) {stop : Nat} (h : stop ≤ x.size) (j : Nat)
+  : anyPairM.loop (cons a x) p (stop + 1) (Nat.succ_le_succ h) 0 (j+1) (j.zero_lt_succ) = x.anyM (p a) j stop >>= fun b => if b then pure true else anyPairM.loop x p stop h 0 1 Nat.zero_lt_one := by
+    conv => lhs; unfold anyPairM.loop
+    conv => rhs; dsimp [anyM]; rewrite [dif_pos h]; unfold anyM.loop
+    simp only [if_pos stop.zero_lt_succ]
+    if hj : j < stop then
+      simp only [dif_pos (Nat.succ_lt_succ hj), dif_pos hj]
+      simp only [getElem_cons_zero, getElem_cons_succ, bind_assoc]
+      apply bind_congr; intro b
+      match b with
+      | true => simp only [ite_true, pure_bind]
+      | false =>
+        simp only [ite_false]
+        rewrite [anyPairM_loop_cons_zero a x p h (j+1)]
+        conv => lhs; lhs; dsimp [anyM]; rw [dif_pos h]
+    else
+      simp only [dif_neg (fun h' => hj (Nat.lt_of_succ_lt_succ h')), dif_neg hj]
+      rewrite [anyPairM_loop_cons_succ a x p h Nat.zero_lt_one]
+      simp only [pure_bind, ite_false]
+termination_by _ => stop - j
+
+@[simp]
+theorem anyPairM_empty (p : α → α → m Bool) {start stop : Nat} : anyPairM #[] p start stop = pure false := by
+  dsimp [anyPairM]
+  simp only [size_toArray, List.length_nil]
+  if h : stop ≤ 0 then
+    rewrite [dif_pos h]
+    exact anyPairM_loop_empty p h start.lt_succ_self
+  else
+    rewrite [dif_neg h]
+    exact anyPairM_loop_empty p .refl start.lt_succ_self
+
+theorem anyPairM_cons_succ (a : α) (x : Array α) (p : α → α → m Bool) {start stop : Nat} : anyPairM (cons a x) p (start + 1) (stop + 1) = anyPairM x p start stop := by
+  dsimp [anyPairM]
+  if h : stop ≤ x.size then
+    rewrite [dif_pos (Nat.succ_le_succ h), dif_pos h]
+    exact anyPairM_loop_cons_succ a x p h start.lt_succ_self
+  else
+    rewrite [dif_neg fun h' => h (Nat.le_of_succ_le_succ h'), dif_neg h]
+    exact anyPairM_loop_cons_succ a x p .refl start.lt_succ_self
+
+theorem anyPairM_cons_zero [LawfulMonad m] (a : α) (x : Array α) (p : α → α → m Bool) {stop : Nat} : anyPairM (cons a x) p 0 (stop + 1) = anyM (p a) x 0 stop >>= fun b => if b then return true else anyPairM x p 0 stop := by
+  dsimp [anyPairM]
+  if h : stop ≤ x.size then
+    rewrite [dif_pos (Nat.succ_le_succ h), dif_pos h]
+    exact anyPairM_loop_cons_zero a x p h 0
+  else
+    rewrite [dif_neg fun h' => h (Nat.le_of_succ_le_succ h'), dif_neg h]
+    apply Eq.trans <| anyPairM_loop_cons_zero a x p .refl 0
+    apply congrFun; apply congrArg
+    dsimp [anyM]
+    simp only [dif_pos x.size.le_refl, dif_neg h]
+
+theorem anyPairM_cons [LawfulMonad m] (a : α) (x : Array α) (p : α → α → m Bool) : anyPairM (cons a x) p = anyM (p a) x >>= fun b => if b then return true else anyPairM x p :=
+  anyPairM_cons_zero a x p
+
+@[simp]
+theorem anyPair_empty (p : α → α → Bool) {start stop : Nat} : anyPair #[] p start stop = false :=
+  anyPairM_empty (m:=Id) p
+
+theorem anyPair_cons_succ (a : α) (x : Array α) (p : α → α → Bool) {start stop : Nat} : anyPair (cons a x) p (start + 1) (stop + 1) = anyPair x p start stop :=
+  anyPairM_cons_succ (m:=Id) a x p
+
+theorem anyPair_cons_zero (a : α) (x : Array α) (p : α → α → Bool) {stop : Nat} : anyPair (cons a x) p 0 (stop + 1) = (any x (p a) 0 stop || anyPair x p 0 stop) := by
+  apply Eq.trans <| anyPairM_cons_zero (m:=Id) a x p
+  conv =>
+    lhs; change if any x (p a) 0 stop = true then true else anyPair x p 0 stop
+  match any x (p a) 0 stop with
+  | true => simp only [ite_true, Bool.true_or]
+  | false => simp only [ite_false, Bool.false_or]
+
+@[simp]
+theorem anyPair_cons (a : α) (x : Array α) (p : α → α → Bool) : anyPair (cons a x) p = (any x (p a) || anyPair x p) :=
+  anyPair_cons_zero a x p
+
+end Any
+
+
+/-! ### Declarations about `Array.Nodup` -/
+
+section Nodup
+
+variable [DecidableEq α]
+
+/--
+`Array.Nodup x` ensures that `x : Array α` has no duplicate in its elements.
+This is an `Array`-counterpart of `List.Nodup`, though it requires `DecidableEq α` in the same spirit of `Membership`.
+-/
+def Nodup (x : Array α) : Prop :=
+  x.anyPair BEq.beq = false
+
+instance Nodup.decidable (x : Array α) : Decidable x.Nodup :=
+  inferInstanceAs <| Decidable (x.anyPair BEq.beq = false)
+
+@[simp]
+theorem nodup_empty : Nodup (#[] : Array α) := by
+  dsimp [Nodup]; exact anyPair_empty BEq.beq
+
+@[simp]
+theorem nodup_cons {a : α} {x : Array α} : Nodup (cons a x) ↔ a ∉ x ∧ Nodup x := by
+  dsimp [Nodup]
+  conv =>
+    pattern a ∉ x; change ¬(x.any (BEq.beq a) = true); rw [Bool.not_eq_true]
+  rewrite [anyPair_cons_zero]
+  match x.any (BEq.beq a) with
+  | true => simp only [Bool.true_or, false_and]
+  | false => simp only [Bool.false_or, true_and]
+
+end Nodup
+
+end Array
